a version of general operational spec for instantiation

theories/iris_host.v
@@ -16,15 +16,15 @@ Definition reduce := @reduce host_function host_instance.
 Definition host_val := val.
 
 (* Domain of the variable instantiation store *)
-Definition vi := nat.
+Definition vi := N.
 
-(* variable instantiation store *)
-Definition vi_store := gmap vi (list module_export).
+(* variable instantiation store. *)
+Definition vi_store := gmap vi module_export.
 
 Definition module_decl := module.
 
-(* an import is specified by giving the index of the instance to the module_export and a name given by the string *)
-Definition vimp : Type := vi * (seq.seq Byte.byte).
+(* an import is specified by giving the index of the instance to the module_export and a second index in the list*)
+Definition vimp : Type := vi.
 
 (* There is only one instance declaration instruction: instantiating a module.
    ID_instantiate vi vm vimps is supposed to instantiate the module vmth module
@@ -32,7 +32,7 @@ Definition vimp : Type := vi * (seq.seq Byte.byte).
    and store the list of exports in the vi_store for future use.
  *)
 Inductive inst_decl: Type :=
-  ID_instantiate: vi -> nat -> list vimp -> inst_decl.
+  ID_instantiate: list vi -> N -> list vimp -> inst_decl.
 
 Definition host_config : Type := store_record * vi_store * (list module) * (list inst_decl) * (list administrative_instruction).
 
@@ -45,19 +45,28 @@ Definition map_start (start: option nat) : list administrative_instruction :=
   | None => []
   end.
 
-Fixpoint lookup_export vexts name : option module_export_desc :=
-  match vexts with
-  | [] => None
-  | e :: vexts' => if e.(modexp_name) == name then Some e.(modexp_desc)
-                                            else lookup_export vexts' name
+Definition lookup_export_vi (vis: vi_store) (vimp: vimp) : option module_export:=
+  vis !! vimp.
+  (*
+  let (vindex, vname) := vimp in
+  match vis !! vindex with
+  | Some vexts => vexts !! (N.to_nat vname)
+  | None => None
+  end.*)
+
+(* some kind of folding on 2 lists *)
+Fixpoint insert_exports (vis: vi_store) (iexps: list vi) (exps: list module_export) : option vi_store :=
+  match iexps with
+  | [::] => Some vis
+  | i :: iexps' => match exps with
+                 | [::] => None
+                 | exp :: exps' => match (insert_exports vis iexps' exps') with
+                                 | Some vis' => Some (<[ i := exp ]> vis')
+                                 | None => None
+                                 end
+                 end
   end.
 
-Definition lookup_export_vi (vis: vi_store) (vimp: vimp) : option module_export_desc :=
-  let (vi, vname) := vimp in
-  match vis !! vi with
-  | Some vexts => lookup_export vexts vname
-  | None => None
-  end.
 
 Definition empty_instance := Build_instance [::] [::] [::] [::] [::].
 Definition empty_frame := Build_frame [::] empty_instance.
@@ -65,14 +74,26 @@ Definition empty_frame := Build_frame [::] empty_instance.
 (* Dummy *)
 Parameter hs: host_state host_instance.
 
+(* Note that instantiation takes imports as module_export_desc but gives exports as module_export (i.e. with a name). *)
+Print instantiation.instantiate.
+
+Print module_export.
+
+Print alloc_module.
+
+
+
+
 Inductive host_reduce: host_config -> host_config -> Prop :=
-| HR_host_step: forall s vis m vi vm vimps imps s' vis' ms idecs' inst exps start vs,
-    ms !! vm = Some m ->
+| HR_host_step: forall s (vis: vi_store) m (viexps: list vi) vm vimps imps imp_descs s' vis' ms idecs' inst (exps: list module_export) start vs,
+    ms !! (N.to_nat vm) = Some m ->
     those ((lookup_export_vi vis) <$> vimps) = Some imps ->
-    instantiate s m imps ((s', inst, exps), start) ->
+    map (fun imp => imp.(modexp_desc)) imps = imp_descs ->
+    instantiate s m imp_descs ((s', inst, exps), start) ->
+    length viexps = length exps ->
     const_list vs ->
-    vis' = <[ vi := exps ]> vis ->
-    host_reduce (s, vis, ms, (ID_instantiate vi vm vimps) :: idecs', vs) (s', vis', ms, idecs', map_start start)
+    insert_exports vis viexps exps = Some vis' ->
+    host_reduce (s, vis, ms, (ID_instantiate viexps vm vimps) :: idecs', vs) (s', vis', ms, idecs', map_start start)
 | HR_wasm_step: forall s vis ms idecs s' es es' hs',
     (* No reentrancy and no host functions, so hs should just be dummy *)
     opsem.reduce hs s empty_frame es hs' s' empty_frame es' ->
@@ -118,9 +139,10 @@ Definition prim_step (e : host_expr) (s : state) (os : list observation) (e' : h
   let '(hes', wes') := e' in
     host_reduce (ws, vis, ms, hes, wes) (ws', vis', ms', hes', wes') /\ os = [] /\ fork_es' = [].
 
+
 Lemma to_of_val v : to_val (of_val v) = Some v.
 Proof.
-  destruct 0 => //; move:l; elim => //=; move => ? ? IH; by rewrite IH => //.
+  by apply iris.to_of_val.
 Qed.
 
 Lemma of_to_val e v : to_val e = Some v → of_val v = e.
@@ -152,38 +174,12 @@ Canonical Structure wasm_host_lang := Language wasm_host_mixin.
 
 Implicit Type σ : state.
 
-(*
-Class wfuncG Σ := WFuncG {
-  func_invG :> invGS Σ;
-  func_gen_hsG :> gen_heapGS N function_closure Σ;
-}.
-
-Class wtabG Σ := WTabG {
-  tab_gen_hsG :> gen_heapGS (N*N) funcelem Σ;
-}.
-
-Class wmemG Σ := WMemG {
-  mem_gen_hsG :> gen_heapGS (N*N) byte Σ;
-}.
-
-Class wmemsizeG Σ := WMemsizeG {
-  memsize_gen_hsG :> gen_heapGS N N Σ;
-}.
-
-Class wglobG Σ := WGlobG {
-  glob_gen_hsG :> gen_heapGS N global Σ;
-}.
-
-Class wframeG Σ := WFrameG {
-  locs_gen_hsG :> ghost_mapG Σ unit frame;
-}.
-*)
 Require Export iris_wp_def.
 
 (* The host expands the memory model of Wasm by vi_store and a list of module declarations. *)
 
 Class hvisG Σ := HVisG {
-  vis_genG :> ghost_mapG Σ nat (list module_export)
+  vis_genG :> ghost_mapG Σ N module_export
 }.
 
 Class hmsG Σ := HMsG {
@@ -196,7 +192,10 @@ Definition frameGName : positive := 10%positive.
 Definition visGName : positive := 11%positive.
 Definition msGName : positive := 12%positive.
 
-Definition proph_id := positive. (* ??? *)
+Definition proph_id := positive. (* still have no idea about what this is *)
+
+Instance eqdecision_vi: EqDecision vi.
+Proof. move => n n'. unfold Decision. by decidable_equality. Qed.
 
 Instance eqdecision_frame: EqDecision frame.
 Proof. decidable_equality. Qed.
@@ -204,7 +203,20 @@ Proof. decidable_equality. Qed.
 Instance eqdecision_module: EqDecision module.
 Proof. move => m m'. unfold Decision. by decidable_equality. Qed.
 
-Global Instance host_heapG_irisG `{!wfuncG Σ, !wtabG Σ, !wmemG Σ, !wmemsizeG Σ, !wglobG Σ, !wframeG Σ, !hvisG Σ, !hmsG Σ} : weakestpre.irisGS wasm_host_lang Σ := {
+Instance eqdecision_module_export: EqDecision (list module_export).
+Proof. decidable_equality. Qed.
+
+Notation " n ↪[vis]{ q } v" := (ghost_map_elem (V := module_export) visGName n q v%V)
+                           (at level 20, q at level 5, format " n ↪[vis]{ q } v") .
+Notation " n ↪[vis] v" := (ghost_map_elem (V := module_export) visGName n (DfracOwn 1) v%V)
+                          (at level 20, format " n ↪[vis] v").
+
+Notation " n ↪[mods]{ q } v" := (ghost_map_elem (V := module) msGName n q v%V)
+                           (at level 20, q at level 5, format " n ↪[mods]{ q } v") .
+Notation " n ↪[mods] v" := (ghost_map_elem (V := module) msGName n (DfracOwn 1) v%V)
+                            (at level 20, format " n ↪[mods] v").
+
+Global Instance host_heapG_irisG `{!wfuncG Σ, !wtabG Σ, !wtabsizeG Σ, !wmemG Σ, !wmemsizeG Σ, !wglobG Σ, !wframeG Σ, !hvisG Σ, !hmsG Σ} : weakestpre.irisGS wasm_host_lang Σ := {
   iris_invGS := func_invG; (* ??? *)
   state_interp σ _ κs _ :=
     let: (s, vis, ms) := σ in
@@ -216,7 +228,8 @@ Global Instance host_heapG_irisG `{!wfuncG Σ, !wtabG Σ, !wmemG Σ, !wmemsizeG 
       (ghost_map_auth msGName 1 (gmap_of_list ms)) ∗
       (* Should this really be here, though? *)
       (ghost_map_auth frameGName 1 (<[ tt := empty_frame ]> ∅)) ∗ 
-      (gen_heap_interp (gmap_of_list (fmap mem_length s.(s_mems))))
+      (gen_heap_interp (gmap_of_list (fmap mem_length s.(s_mems)))) ∗
+      (gen_heap_interp (gmap_of_list (fmap tab_size s.(s_tables))))
     )%I;
     num_laters_per_step _ := 0;
     fork_post _ := True%I;
@@ -227,7 +240,7 @@ Global Instance host_heapG_irisG `{!wfuncG Σ, !wtabG Σ, !wmemG Σ, !wmemsizeG 
 
 
 Section host_lifting.
-Context `{!wfuncG Σ, !wtabG Σ, !wmemG Σ, !wmemsizeG Σ, !wglobG Σ, !wframeG Σ, !hvisG Σ, !hmsG Σ}.
+Context `{!wfuncG Σ, !wtabG Σ, !wtabsizeG Σ, !wmemG Σ, !wmemsizeG Σ, !wglobG Σ, !wframeG Σ, !hvisG Σ, !hmsG Σ}.
 
 
 (* adding this would nullify all lemmas in weakestpre -- why? Is this not the 
@@ -260,6 +273,7 @@ Inductive host_wasm_expr_valid : list administrative_instruction -> Prop :=
 | HWEV_const: forall es,
     const_list es ->
     host_wasm_expr_valid es
+(* Trap is also a possibility *)
 | HWEV_trap:
     host_wasm_expr_valid [AI_trap]
 | HWEV_invoke: forall n,
@@ -269,6 +283,8 @@ Inductive host_wasm_expr_valid : list administrative_instruction -> Prop :=
 
 Hint Constructors host_wasm_expr_valid.
 
+
+
 (* Any possible wasm expression as defined above reduces independently from the frame. *)
 Lemma hwev_reduce_ignore_frame es hs ws f1 f2 hs' ws' f' es':
   host_wasm_expr_valid es ->
@@ -277,7 +293,9 @@ Lemma hwev_reduce_ignore_frame es hs ws f1 f2 hs' ws' f' es':
 Proof.
   move => Hhwev Hred.
   inversion Hhwev; subst; clear Hhwev.
+  (* values *)
   - by apply values_no_reduce in Hred.
+  (* trap *)
   - by apply test_no_reduce_trap in Hred.
   - remember [AI_invoke n] as es0. induction Hred; subst => //=.
     + inversion H; subst; clear H => //=; try by do 3 destruct vs => //.
@@ -296,6 +314,7 @@ Proof.
       inversion H0; subst; clear H0.
       simpl; rewrite cats0.
       by apply IHHred.
+  (* local *)
   - remember [AI_local n f es0] as es1. induction Hred => //=.
     + inversion H; subst; clear H => //=; try by do 3 destruct vs => //.
       * inversion H2; subst; clear H2.
@@ -321,7 +340,9 @@ Proof.
       by apply IHHred.
     + by apply r_local.
 Qed.
-      
+
+
+
 (* The set of possible wasm expressions is closed wrt reduce. *)
 Lemma hwev_reduce_closed hs ws f es hs' ws' f' es':
   host_wasm_expr_valid es ->
@@ -360,7 +381,9 @@ Proof.
       simpl; rewrite cats0.
       by apply IHHred.
 Qed.
-      
+
+
+
 (* Lifting reduction of valid wasm expressions to host configurations. *)
 Lemma reducible_lift es ws vis ms:
   host_wasm_expr_valid es ->
@@ -396,7 +419,7 @@ Proof.
   destruct (iris.to_val es) eqn: Hes => //=.
   iIntros ([[ws vis] ms] ns κ κs nt) "Hσ".
   iSpecialize ("Hwp" $! (hs, ws, [::], empty_instance) ns κ κs nt).
-  iDestruct "Hσ" as "(Hwf & Hwt & Hwm & Hwg & Hvis & Hms & Hframe & Hmsize)".
+  iDestruct "Hσ" as "(Hwf & Hwt & Hwm & Hwg & Hvis & Hms & Hframe & Hmsize & Htsize)".
   iSpecialize ("Hwp" with "[$]").
   iMod "Hwp" as "(%Hred & Hwp)".
   iModIntro.
@@ -415,7 +438,7 @@ Proof.
     iModIntro.
     iMod "Hwp".
     iModIntro.
-    iDestruct "Hwp" as "((Hwf & Hwt & Hwm & Hwg & Hwframe & Hmsize) & Hwp)".
+    iDestruct "Hwp" as "((Hwf & Hwt & Hwm & Hwg & Hwframe & Hmsize & Htsize) & Hwp)".
     iDestruct "Hwp" as (f) "(Hf & Hwp & ?)".
     iFrame.
     iSplit => //.
@@ -423,7 +446,658 @@ Proof.
     iApply "Hwp".
     by iApply "Hf".
 Qed.
+
+End host_lifting.
+
+
+
+Section Instantiation_spec_operational.
+
+Context `{!wfuncG Σ, !wtabG Σ, !wtabsizeG Σ, !wmemG Σ, !wmemsizeG Σ, !wglobG Σ, !wframeG Σ, !hvisG Σ, !hmsG Σ}.
+
+Print module_export_desc.
+
+(* The newly allocated resources due to instantiation. *)
+Definition module_inst_resources_func (mfuncs: list module_func) (inst: instance) (addrs: list N) : iProp Σ :=
+  ([∗ list] f; addr ∈ mfuncs; addrs,
+   (* Allocated wasm resources *)
+     addr ↦[wf] (FC_func_native
+                             inst
+                             (nth match f.(modfunc_type) with
+                                 | Mk_typeidx k => k
+                                 end (inst.(inst_types)) (Tf [] []))
+                             f.(modfunc_locals)
+                             f.(modfunc_body))
+  )%I.
+
+
+Definition module_inst_resources_tab (mtabs: list module_table) (addrs: list N) : iProp Σ :=
+  ([∗ list] tab; addr ∈ mtabs; addrs,
+    addr ↦[wtblock] (match tab.(modtab_type).(tt_limits) with
+                            | {| lim_min := min; lim_max := omax |} =>
+                                 (Build_tableinst
+                                   (repeat None (ssrnat.nat_of_bin min)))
+                                   (omax)
+                       end)
+  )%I.
+
+
+Definition module_inst_resources_mem (mmems: list memory_type) (addrs: list N) : iProp Σ := 
+  ([∗ list] mem; addr ∈ mmems; addrs,
+    addr ↦[wmblock] (match mem with
+                                 | {| lim_min:= min; lim_max := omax |} =>
+                                   Build_memory
+                                     {| ml_init := #00%byte; ml_data := repeat #00%byte (N.to_nat min) |}
+                                     (omax)
+                                  end)
+  ).
+
+Definition module_inst_resources_glob (mglobs: list module_glob) (val_addrs: list (value * N)) : iProp Σ :=
+  ([∗ list] g; val_addr ∈ mglobs; val_addrs,
+    let '(g_init, addr) := val_addr in
+    addr ↦[wg] (Build_global
+                               (g.(modglob_type).(tg_mut))
+                               g_init
+                            )
+  ).
+
+
+Print module_export_desc.
+
+Print fold_left.
+
+Print module.
+
+(* The collection of the four types of newly allocated resources *)
+Definition module_inst_resources_wasm (m: module) (inst: instance) (wfaddr wtaddr wmaddr: list N) (wgval_addr: list (value * N)) : iProp Σ :=
+  (module_inst_resources_func m.(mod_funcs) inst wfaddr ∗
+  module_inst_resources_tab m.(mod_tables) wtaddr ∗
+  module_inst_resources_mem m.(mod_mems) wmaddr ∗                        
+  module_inst_resources_glob m.(mod_globals) wgval_addr)%I.
+
+(* Resources in the host vis store for the imports *)
+Definition import_resources_host (hs_imps: list vimp) (v_imps : list module_export): iProp Σ :=
+  [∗ list] i ↦ hs_imp; v_imp ∈ hs_imps; v_imps,
+  hs_imp ↪[vis] v_imp.
+
+(*
+Definition export_ownership_host (hs_exps: list vi) : iProp Σ :=
+  [∗ list] i ↦ hs_exp ∈ hs_exps,
+  ∃ hv, hs_exp ↪[vis] hv.
+*)
+
+
+Print instantiation.instantiate.
+
+Print external_typing.
+
+Print instantiate_globals.
+
+Definition instantiate_globals := instantiate_globals host_function host_instance.
+
+Search module_export.
+
+Print module_export_typer.
+
+Print alloc_module.
+
+Print export_get_v_ext.
+
+Print alloc_func.
+
+Print module_export.
+
+Print module_export_desc.
+
+Print module_typing.
+
+Print ext_t_funcs.
+
+Print map.
+
+Print extern_t.
+
+(* Resources in the Wasm store, corresponding to those referred by the host vis store. This needs to also type-check
+   with the module import. *)
+Definition import_resources_wasm_typecheck (v_imps: list module_export) (t_imps: list extern_t): iProp Σ :=
+  [∗ list] i ↦ v; t ∈ v_imps; t_imps,
+  match v.(modexp_desc) with
+  | MED_func (Mk_funcidx i) => ((∃ cl q, N.of_nat i ↦[wf]{ q } cl ∗ ⌜ t = ET_func (cl_type cl) ⌝)%I)
+  | MED_table (Mk_tableidx i) => (∃ tab, N.of_nat i ↦[wtblock] tab ∗ True) (* table type is currently not a part of the resources, so we cannot know this *)
+  | MED_mem (Mk_memidx i) => (∃ mem, N.of_nat i ↦[wmblock] mem ∗ True) (* same for memories *)
+  | MED_global (Mk_globalidx i) => (∃ g q gt, N.of_nat i ↦[wg]{ q } g ∗ ⌜ t = ET_glob gt /\ global_agree g gt ⌝)
+  end.
+
+(*
+Print module.
+
+Print module_export.
+
+Print module_export_desc.
+
+Print module_import.
+
+Print import_desc.
+
+
+(* Getting the count of each type of imports from a module. This is to calculate the correct shift for indices of the exports in the Wasm store later.*)
+Definition get_import_func_count (m: module) := length (pmap (fun x => match x.(imp_desc) with
+                                                                   | ID_func id => Some id
+                                                                   | _ => None
+                                                                    end) m.(mod_imports)).
+
+Definition get_import_table_count (m: module) := length (pmap (fun x => match x.(imp_desc) with
+                                                                   | ID_table id => Some id
+                                                                   | _ => None
+                                                                    end) m.(mod_imports)).
+Definition get_import_mem_count (m: module) := length (pmap (fun x => match x.(imp_desc) with
+                                                                   | ID_mem id => Some id
+                                                                   | _ => None
+                                                                    end) m.(mod_imports)).
+Definition get_import_global_count (m: module) := length (pmap (fun x => match x.(imp_desc) with
+                                                                   | ID_global id => Some id
+                                                                   | _ => None
+                                                                    end) m.(mod_imports)).
+
+(* The expected host resources that we should be getting from the module exports after instantiation. 
+
+   Note that an export of index i is in fact the (i-n)th definition within the module itself (where n is the number of 
+   imports of the same kind used by the module); so the correct index in the Wasm store should be the starting 
+   offset + (i-n)).
+
+   It is true that we can existentially quantify over the addresses to simplify this definition, and this might have 
+   been an overkill. However, that loses the information that the newly allocated elements are guaranteed to be a 
+   contiguous block (or maybe that is unimportant).
+*)                                     
+Definition export_resources_host (m: module) (hs_exps: list vi) (nf nt nm ng: nat) : iProp Σ :=
+  [∗ list] i ↦ hs_exp; m_exp ∈ hs_exps; m.(mod_exports),
+      N.of_nat i ↪[vis] match m_exp.(modexp_desc) with
+               | MED_func (Mk_funcidx i) => {| modexp_name := m_exp.(modexp_name); modexp_desc := MED_func (Mk_funcidx (nf + i - get_import_func_count m)) |}
+               | MED_table (Mk_tableidx i) => {| modexp_name := m_exp.(modexp_name); modexp_desc := MED_table (Mk_tableidx (nt + i - get_import_table_count m)) |}
+               | MED_mem (Mk_memidx i) => {| modexp_name := m_exp.(modexp_name); modexp_desc := MED_mem (Mk_memidx (nm + i - get_import_mem_count m)) |}
+               | MED_global (Mk_globalidx i) => {| modexp_name := m_exp.(modexp_name); modexp_desc := MED_global (Mk_globalidx (ng + i - get_import_global_count m)) |}
+                        end.
+*)
+
+Definition exp_default := MED_func (Mk_funcidx 0).
+
+(* The resources for module exports. This is a bit more complicated since it is allowed to export the imported elements,
+   adding another case to be considered. *)
+Definition module_export_resources_host (v_imps: list module_export) (hs_exps: list vi) (m_exps: list module_export) (wfaddr wtaddr wmaddr wgaddr: list N) : iProp Σ :=
+  (* For each export, if it is actually imported by the module (i.e. not newly allocated), then we should have the
+     host vis points to the old location; otherwise it should point to the address as specified in one of the four
+     address lists. 
+
+     We implement the above by first construct the list of exports corresponding to all the entities in the module
+     (i.e. imports + new declarations), then lookup from this list to find the correct export.
+*)
+  let wf_exps := ((pmap (fun x => match x.(modexp_desc) with
+                              | MED_func _ => Some x.(modexp_desc)
+                              | _ => None
+                              end) v_imps) ++ (map (fun addr => MED_func (Mk_funcidx (N.to_nat addr))) wfaddr)) in 
+  let wt_exps := ((pmap (fun x => match x.(modexp_desc) with
+                              | MED_table _ => Some x.(modexp_desc)
+                              | _ => None
+                               end) v_imps) ++ (map (fun addr => MED_table (Mk_tableidx (N.to_nat addr))) wtaddr)) in
+  let wm_exps := ((pmap (fun x => match x.(modexp_desc) with
+                              | MED_mem _ => Some x.(modexp_desc)
+                              | _ => None
+                               end) v_imps) ++ (map (fun addr => MED_mem (Mk_memidx (N.to_nat addr))) wmaddr)) in
+  let wg_exps := ((pmap (fun x => match x.(modexp_desc) with
+                              | MED_global _ => Some x.(modexp_desc)
+                              | _ => None
+                               end) v_imps) ++ (map (fun addr => MED_global (Mk_globalidx (N.to_nat addr))) wgaddr)) in
+  [∗ list] hs_exp; m_exp ∈ hs_exps; m_exps,
+                                    ∃ name, hs_exp ↪[vis] Build_module_export name
+                                                   (match m_exp.(modexp_desc) with
+                                                   | MED_func (Mk_funcidx n) => nth n wf_exps exp_default
+                                                   | MED_table (Mk_tableidx n) => nth n wt_exps exp_default
+                                                   | MED_mem (Mk_memidx n) => nth n wm_exps exp_default
+                                                   | MED_global (Mk_globalidx n) => nth n wg_exps exp_default
+                                                   end
+                                                     ).
+
+
+
+Lemma instantiation_spec_operational (s: stuckness) E (hs_mod: N) (hs_imps: list vimp) (v_imps: list module_export) (hs_exps: list vi) (m: module) t_imps t_exps:
+  module_typing m t_imps t_exps ->
+  hs_mod ↪[mods] m -∗
+  import_resources_host hs_imps v_imps -∗
+  import_resources_wasm_typecheck v_imps t_imps -∗
+  WP (([:: ID_instantiate hs_exps hs_mod hs_imps], [::]): host_expr) @ s; E
+  {{ v, hs_mod ↪[mods] m ∗
+        import_resources_host hs_imps v_imps ∗ (* vis, for the imports stored in host *)
+        import_resources_wasm_typecheck v_imps t_imps ∗ (* locations in the wasm store and type-checks *)
+        ∃ inst wfaddr wtaddr wmaddr wgval_addr,
+          module_inst_resources_wasm m inst wfaddr wtaddr wmaddr wgval_addr ∗ (* allocated wasm resources *)
+          module_export_resources_host v_imps hs_exps m.(mod_exports) wfaddr wtaddr wmaddr (map (fun x => x.2) wgval_addr)
+  }}.
+Proof.
+  (*
+  move => Hmodtype.
+  iIntros "Hmod Himphost Himpwasm Hexphost".
   
+  repeat rewrite weakestpre.wp_unfold /weakestpre.wp_pre /=.
+  
+  iIntros ([[ws vis] ms] ns κ κs nt) "Hσ".
+  iDestruct "Hσ" as "(Hwf & Hwt & Hwm & Hwg & Hvis & Hms & Hframe & Hmsize & Htsize)".
+
+  (* Reflecting the assertions back *)
+  iDestruct (ghost_map_lookup with "Hms Hmod") as "%Hmod".
+  unfold import_resources_host, big_opL.
+  Print big_sepL2.
+  unfold big_sepL2.
+  Search big_sepL2.
+  Print ghost_map_lookup.
+  iDestruct (ghost_map_lookup with "Hvis Himphost") as "%Himphost".
+  Search ghost_map_elem big_opM.
+  Search big_opL big_opM.
+
+  Search gmap list.
+  
+  iDestruct (ghost_map_lookup_big with "Hvis Himphost") as "%Himphost".
+
+  (* The key is to prove that the instantiate predicate holds with the premises given. *)
+  assert (exists ws_res inst_res v_exps ostart, (instantiate ws m v_imps ((ws_res, inst_res, v_exps), ostart))) as Hinst.
+  {
+    admit.
+  }
+
+  destruct Hinst as [[[[ws_res inst_res] v_exps] ostart] Hinst].
+  
+  iApply fupd_mask_intro; first by set_solver.
+
+  iIntros "Hmask".
+  iSplit.
+  
+  - destruct s => //.
+    iPureIntro.
+    unfold language.reducible.
+      
+    exists [], (([::], [::]): host_expr), (ws2,
+                                    <[ 0 := [:: Build_module_export (list_byte_of_string "add") (MED_func (Mk_funcidx 0))]]>
+                                    (<[ 1 := [:: Build_module_export (list_byte_of_string "f") (MED_func (Mk_funcidx 1))]]> vis) ,
+                                    ms), [].
+    unfold prim_step.
+    repeat split => //.
+    admit.
+    (*
+    eapply HR_host_step => //.
+    by rewrite gmap_of_list_lookup in Hmods.
+*)
+        
+  - iIntros ([hes' wes'] [[ws3 vis3] ms3] efs HStep).
+    destruct HStep as [HStep [-> ->]].
+    inversion HStep; subst; clear HStep.
+    iIntros "!>!>!>".
+    iMod "Hmask".
+    iModIntro.
+*)
+Admitted.
+  
+End Instantiation_spec_operational.
+
+
+(* Examples *)
+
+Section Example_Add.
+
+Definition Add_module :=
+  Build_module
+    (* Function types *) [:: (Tf [::T_i32; T_i32] [::T_i32]) ]
+    (* Functions *) [:: Build_module_func
+                       (* Type signature, referencing from the function type components *) (Mk_typeidx 0)
+                       (* List of local variable types to be used -- none for the addition here *) [::]
+                       (* Function body *) [:: BI_get_local 0; BI_get_local 1; BI_binop T_i32 (Binop_i BOI_add)]
+                       ]
+    (* Tables *) [::]
+    (* Memories *) [::]
+    (* Globals *) [::]
+    (* Table initializers *) [::]
+    (* Memory initializers *) [::]
+    (* Start function *) None
+    (* Imports *) [::]
+    (* Exports *) [:: Build_module_export
+                     (* export name *) (list_byte_of_string "add")
+                     (* export description *) (MED_func (Mk_funcidx 0))
+                     ].
+
+Definition xx i := (VAL_int32 (Wasm_int.int_of_Z i32m i)).
+
+Definition M2 :=
+  Build_module
+    (* Function types *) [:: (Tf [::T_i32; T_i32] [::T_i32]); (Tf [::] [::T_i32]) ]
+    (* Functions *) [:: Build_module_func
+                       (* Type signature, referencing from the function type components *) (Mk_typeidx 1)
+                       (* List of local variable types to be used -- none for the addition here *) [::]
+                       (* Function body *) [:: BI_const (xx 13); BI_const (xx 2); BI_call 0]
+                       (* Note that the imports take precedence, i.e. the imported function is the 0th function, and
+                          this function is the 1st function instead. *)
+                       ]
+    (* Tables *) [::]
+    (* Memories *) [::]
+    (* Globals *) [::]
+    (* Table initializers *) [::]
+    (* Memory initializers *) [::]
+    (* Start function *) (* This would actually not work -- the start function must have an empty function type *)
+                  (* (Some (Build_module_start (Mk_funcidx 1))) *)
+                  None
+    (* Imports *) [:: Build_module_import
+                     (* import module name (superfluous) *) (list_byte_of_string "Add_module")
+                     (* import function name (superfluous) *) (list_byte_of_string "add")
+                     (* import type description *) (ID_func 0)
+                     ]
+    (* Exports *) [:: Build_module_export
+                     (* export name *) (list_byte_of_string "f")
+                     (* export description *) (MED_func (Mk_funcidx 1))
+                     ].
+
+Definition module_decls := [:: Add_module; M2].
+
+Definition add_program_instantiate :=
+  [:: ID_instantiate 0 0 [::];
+  (* The above exports the function 'add' to the 0th vi store of the host, which contains a list of exports consisting of
+     only one function -- the add function. *)
+  ID_instantiate 1 1 [:: (0, (list_byte_of_string "add"))]].
+  
+End Example_Add.
+
+
+
+
+
+
+(* verify that both modules are well-typed *)
+Lemma add_module_valid: module_typing Add_module [::] [:: ET_func (Tf [::T_i32; T_i32] [::T_i32])].
+Proof.
+  unfold module_typing.
+  (* We have to provide the type of each function and each global in the instantiate module. *)
+  exists [Tf [::T_i32; T_i32] [::T_i32]], [::].
+  simpl.
+  (* Most of the components of the module are empty and can be resolved trivially. *)
+  repeat split; (try by apply Forall2_nil); (try by apply Forall_nil).
+  - (* module_func_typing *)
+    constructor; last by apply Forall2_nil.
+    unfold module_func_typing.
+    repeat split => //=.
+    (* be_typing of the function body *)
+    eapply bet_composition_front; first by apply bet_get_local => //.
+    eapply bet_composition_front with (t2s := [T_i32; T_i32]).
+    + replace [T_i32; T_i32] with ([T_i32] ++ [T_i32]) => //.
+      apply bet_weakening_empty_1.
+      by apply bet_get_local.
+    + apply bet_binop.
+      by constructor.
+  - (* module_export_typing *)
+    constructor; last by apply Forall2_nil.
+    by unfold module_export_typing => /=.
+Qed.
+
+
+Lemma M2_valid: module_typing M2 [:: ET_func (Tf [::T_i32; T_i32] [::T_i32])] [:: ET_func (Tf [::] [::T_i32])].
+Proof.
+  unfold module_typing.
+  exists [::Tf [::] [::T_i32]], [::].
+  simpl.
+  repeat split; (try by apply Forall2_nil); (try by apply Forall_nil).
+  - (* module_func_typing *)
+    constructor; last by apply Forall2_nil.
+    unfold module_func_typing.
+    repeat split => //=.
+    (* be_typing of the function body *)
+    eapply bet_composition_front; first by apply bet_const => //.
+    eapply bet_composition_front with (t2s := [T_i32; T_i32]) => /=.
+    + replace [T_i32; T_i32] with ([T_i32] ++ [T_i32]) => //.
+      apply bet_weakening_empty_1.
+      by apply bet_const.
+    + by apply bet_call => //.
+  - (* module_import_typing *)
+    unfold module_import_typing => /=.
+    by constructor => //. 
+  - (* module_export_typing *)
+    constructor; last by apply Forall2_nil.
+    by unfold module_export_typing => /=.    
+Qed.
+
+
+Print instantiation.instantiate.
+Print module_export.
+Print module_export_desc.
+
+Print Build_instance.
+Print funcaddr.
+
+Print function_closure.
+
+Print instance.
+
+Lemma Add_module_instantiate_spec ws n inst ws':
+  length (ws.(s_funcs)) = n ->
+  inst = Build_instance [::Tf [::T_i32; T_i32] [::T_i32]] [::(* wait... this is 1-indexed ???? *)n] [::] [::] [::] ->
+  ws' = (Build_store_record
+            (ws.(s_funcs) ++ [::FC_func_native
+                                       inst 
+                                       (Tf [::T_i32; T_i32] [::T_i32]) (* Function type *)
+                                       [::] (* list of local variable types to be created -- none *)
+                                       [BI_get_local 0; BI_get_local 1; BI_binop T_i32 (Binop_i BOI_add)]])
+            ws.(s_tables)
+            ws.(s_mems)
+            ws.(s_globals)) ->
+  instantiate ws Add_module [::]
+              (
+                ws',
+                inst,
+                [:: Build_module_export (list_byte_of_string "add") (MED_func (Mk_funcidx (n)))],
+                (None: option nat)
+              ).
+Proof.
+  move => Hfunclen Hinst Hstore.
+  unfold instantiate, instantiation.instantiate.
+  
+  (* Types of imports and exports. This might be useful to craft a 'spec for a module' *)
+  exists [::], [::ET_func (Tf [::T_i32; T_i32] [::T_i32])].
+  exists hs. (* updated host state... but our host is built on dummyhost -- so this should really be just a dummy *)
+  exists ws'.
+  exists [::], [::], [::]. (* all of these should be empty *)
+  
+  repeat split; (try by apply Forall2_nil); (try by apply Forall_nil).
+  - (* module_typing of the module, proved above *)
+    by apply add_module_valid.
+  - (* alloc_module *)
+    unfold alloc_module => /=.
+    repeat (apply/andP; split => //; try by rewrite Hinst).
+    rewrite Hinst Hstore => /=.
+    apply/eqP.
+    f_equal.
+    rewrite app_length.
+    by rewrite Hfunclen.
+  - (* This seems to be a recursive check that our store is containing the correct memories and tables -- but how
+       are these working exactly when we actually have some non-empty memories/tables? *)
+    simpl.
+    (* potential bug in instantiation *)
+    unfold init_mems => /=.
+    unfold init_tabs => /=.
+    by apply/eqP.    
+Qed.
+
+
+
+Lemma M2_instantiate_spec ws n inst ws' k:
+  k < n ->
+  length (ws.(s_funcs)) = n ->
+  (* So the instance has to contain imported functions as well *)
+  inst = Build_instance [::Tf [::T_i32; T_i32] [::T_i32]; Tf [::] [::T_i32]] [::k; n+1] [::] [::] [::] ->
+  nth_error ws.(s_funcs) k = Some (FC_func_native
+                                       inst (* redundant instance?? *)
+                                       (Tf [::T_i32; T_i32] [::T_i32]) (* Function type *)
+                                       [::] (* list of local variable types to be created -- none *)
+                                       [BI_get_local 0; BI_get_local 1; BI_binop T_i32 (Binop_i BOI_add)]) ->
+  ws' = (Build_store_record
+            (ws.(s_funcs) ++ [::FC_func_native
+                                       inst 
+                                       (Tf [::] [::T_i32]) 
+                                       [::] 
+                                       [ BI_const (xx 13); BI_const (xx 2); BI_call 0]])
+            ws.(s_tables)
+            ws.(s_mems)
+            ws.(s_globals)) ->
+  instantiate ws M2 [::MED_func (Mk_funcidx k)]
+              (
+                ws',
+                inst,
+                [:: Build_module_export (list_byte_of_string "f") (MED_func (Mk_funcidx (n+1)))],
+                (None: option nat)
+              ).
+Proof.
+  move => Hindexsize Hfunclen Hinst Hfuncimport Hstore.
+  unfold instantiate, instantiation.instantiate.
+  
+  exists [::ET_func (Tf [::T_i32; T_i32] [::T_i32])], [::ET_func (Tf [::] [::T_i32])], hs, ws', [::], [::], [::].
+  
+  repeat split; (try by apply Forall2_nil); (try by apply Forall_nil).
+  - (* module_typing of the module, proved above *)
+    by apply M2_valid.
+  - (* external_typing *)
+    constructor => //.
+    econstructor => //.
+    by lias.
+  - (* alloc_module *)
+    unfold alloc_module => /=.
+    repeat (apply/andP; split => //; try by rewrite Hinst).
+    rewrite Hinst Hstore => /=.
+    apply/eqP.
+    repeat f_equal.
+    rewrite app_length.
+    by rewrite Hfunclen.
+  - simpl.
+    unfold init_mems => /=.
+    unfold init_tabs => /=.
+    by apply/eqP.    
+Qed.
+
+(* Currently only states what are the exports we're getting instead of what the specs are.  *)
+Lemma example_add_spec (s: stuckness) E:
+  (* Module declaration resources *)
+  0%N ↪[mods] Add_module -∗
+  1%N ↪[mods] M2 -∗
+  (* original vis resources -- this is required since the instantiation updates these two entries *)
+  0 ↪[vis] ([::]: list module_export) -∗
+  1 ↪[vis] ([::]: list module_export) -∗
+  WP ((add_program_instantiate, [::]): host_expr) @ s; E
+           {{ v, ⌜ v = immV [::] ⌝ ∗
+                   0%N ↪[mods] Add_module ∗
+                   1%N ↪[mods] M2 ∗
+                   (* It now really seems that this exported funcid is a reference to the location in the store *)
+                   0 ↪[vis] [:: Build_module_export (list_byte_of_string "add") (MED_func (Mk_funcidx 0))] ∗
+                   1 ↪[vis] [:: Build_module_export (list_byte_of_string "f") (MED_func (Mk_funcidx 1))] ∗
+                   (∃ k inst1 inst2, k ↪[wf] (FC_func_native
+                                     inst1
+                                     (Tf [::T_i32; T_i32] [::T_i32]) (* Function type *)
+                                     [::] (* list of local variable types to be created -- none *)
+                                     [BI_get_local 0; BI_get_local 1; BI_binop T_i32 (Binop_i BOI_add)]) ∗
+                   k+1 ↪[wf] (FC_func_native
+                                       inst2 
+                                       (Tf [::] [::T_i32]) 
+                                       [::] 
+                                       [ BI_const (xx 13); BI_const (xx 2); BI_call 0]))
+           }}.
+Proof.
+  iIntros "Hmod1 Hmod2 Hmodexp1 Hmodexp2".
+  repeat rewrite weakestpre.wp_unfold /weakestpre.wp_pre /=.
+  
+  iIntros ([[ws vis] ms] ns κ κs nt) "Hσ".
+  iDestruct "Hσ" as "(Hwf & Hwt & Hwm & Hwg & Hvis & Hms & Hframe & Hmsize)".
+  iDestruct (ghost_map_lookup with "Hms Hmod1") as "%Hmod1".
+  iDestruct (ghost_map_lookup with "Hms Hmod2") as "%Hmod2".
+  iDestruct (ghost_map_lookup with "Hvis Hmodexp1") as "%Hmodexp1".
+  iDestruct (ghost_map_lookup with "Hvis Hmodexp2") as "%Hmodexp2".
+
+  remember (length ws.(s_funcs)) as wflen.
+  remember (Build_instance [::Tf [::T_i32; T_i32] [::T_i32]] [::wflen + 1] [::] [::] [::]) as inst1.
+  remember (Build_store_record
+            (ws.(s_funcs) ++ [::FC_func_native
+                                       inst1
+                                       (Tf [::T_i32; T_i32] [::T_i32]) 
+                                       [::] 
+                                       [BI_get_local 0; BI_get_local 1; BI_binop T_i32 (Binop_i BOI_add)]])
+            ws.(s_tables)
+            ws.(s_mems)
+            ws.(s_globals)) as ws1.
+  
+  specialize (Add_module_instantiate_spec ws wflen inst1 ws1) as Hinstantiate1.
+  
+
+  remember (Build_instance [::Tf [::T_i32; T_i32] [::T_i32]; Tf [::] [::T_i32]] [::wflen; wflen+1] [::] [::] [::]) as inst2.
+  remember (Build_store_record
+            (ws.(s_funcs) ++ [::FC_func_native
+                                       inst2
+                                       (Tf [::] [::T_i32]) 
+                                       [::] 
+                                       [ BI_const (xx 13); BI_const (xx 2); BI_call 0]])
+            ws.(s_tables)
+            ws.(s_mems)
+            ws.(s_globals)) as ws2.
+  
+  specialize (M2_instantiate_spec ws1 (wflen+1) inst2 ws2 (wflen)) as Hinstantiate2.
+
+  iApply fupd_mask_intro; first by set_solver.
+
+  iIntros "Hmask".
+  iSplit.
+  
+  - destruct s => //.
+    iPureIntro.
+    unfold language.reducible.
+      
+    exists [], (([::], [::]): host_expr), (ws2,
+                                    <[ 0 := [:: Build_module_export (list_byte_of_string "add") (MED_func (Mk_funcidx 0))]]>
+                                    (<[ 1 := [:: Build_module_export (list_byte_of_string "f") (MED_func (Mk_funcidx 1))]]> vis) ,
+                                    ms), [].
+    unfold prim_step.
+    repeat split => //.
+    admit.
+    (*
+    eapply HR_host_step => //.
+    by rewrite gmap_of_list_lookup in Hmods.
+*)
+        
+  - iIntros ([hes' wes'] [[ws3 vis3] ms3] efs HStep).
+    destruct HStep as [HStep [-> ->]].
+    inversion HStep; subst; clear HStep.
+    iIntros "!>!>!>".
+    iMod "Hmask".
+    iModIntro.
+    (* It's probably a bad idea to iFrame now... *)
+    (*
+    iFrame.
+*)
+      (*
+      iSpecialize ("Hwp" $! wes' (hs', ws2, [::], empty_instance) [::] with "[%]"); first by unfold iris.prim_step.
+      iMod "Hwp".
+      do 2 iModIntro.
+      iFrame.
+      iSplit => //.
+      iApply "IH"; first by apply hwev_reduce_closed in H0.
+      iApply "Hwp".
+      by iApply "Hf".
+*)
+Admitted.
+
+
+
+
+
+Definition build_module_one_func (ft: function_type) (bes: expr) :=
+  Build_module [:: ft] [:: (Build_module_func (Mk_typeidx 0) [::] bes)] [] [] [] [] [] (Some (Build_module_start (Mk_funcidx 0))) [] [].
+
+Print module_typing.
+
+Print module_func_typing.
+
+Print module_func.
+
+Print typeidx.
+
 (*
 Section Host_wp_import.
   (* Host wp must depend on the same memory model as for wasm *)
@@ -453,7 +1127,108 @@ Section Host_wp_import.
 End Host_wp_import.
  *)
 
-  End host_lifting.
 
+(*
+| HR_host_step: forall s vis m vi vm vimps imps s' vis' ms idecs' inst exps start vs,
+    ms !! vm = Some m ->
+    those ((lookup_export_vi vis) <$> vimps) = Some imps ->
+    instantiate s m imps ((s', inst, exps), start) ->
+    const_list vs ->
+    vis' = <[ vi := exps ]> vis ->
+    host_reduce (s, vis, ms, (ID_instantiate vi vm vimps) :: idecs', vs) (s', vis', ms, idecs', map_start start)
+ *)
+Lemma wp_host_inst_func_only (s: stuckness) E (bes: expr) (Φ: iris.val -> iProp Σ) (m: module) (ft: function_type) (es: expr) (impts expts : list extern_t) q:
+  m = build_module_one_func ft es ->
+  module_typing m impts expts ->
+  WP ((to_e_list bes): iris.expr) @ s; E {{ Φ }} -∗
+  (ghost_map_elem msGName 0%N q m)%I -∗
+  (* Instantiating the 0th module and store exports (None) in the 0th resource should result in the expression containing
+     the resulting value of the function body of the start function, with an empty resource generated at the 0th location *)
+  WP (([::ID_instantiate 0 0 [::]], [::]): host_expr) @ s; E {{ v, Φ v ∗ (ghost_map_elem visGName 0 (DfracOwn 1) ([::]: list module_export)) }}.
+Proof.
+  move => Hmodule Hmoduletype.
+  iIntros "Hwp Hmods".
+  repeat rewrite weakestpre.wp_unfold /weakestpre.wp_pre /=.
+  repeat rewrite wp_unfold /wp_pre /=.
+  
+  iIntros ([[ws vis] ms] ns κ κs nt) "Hσ".
+  iDestruct "Hσ" as "(Hwf & Hwt & Hwm & Hwg & Hvis & Hms & Hframe & Hmsize)".
+  iDestruct (ghost_map_lookup with "Hms Hmods") as "%Hmods".
+  
+  assert (exists s' inst, (instantiate ws m [::] ((s', inst, [::]), (Some 0)))) as [ws' Hinst].
+  {
+    (*
+    destruct ws.
+    exists Build_store_record (s.(s_funcs) ++ (Build_module_func (Mk_typeidx 0) [::] bes)) s.(s_tables) s.(s_mems) s.(s_globals).
+    repeat split; unfold all2.*)
+    admit.
+  }
+  destruct Hinst as [inst Hinstantiate].
+  destruct (iris.to_val (to_e_list bes)) eqn: Hes => //.
+  - (* Can a function body be consisted of only a list of consts? *)
+    iMod "Hwp".
+    iApply fupd_mask_intro; first by set_solver.
+    iIntros "Hmask".
+    iSplit.
+    + iPureIntro.
+      destruct s => //.
+      econstructor.
+      Search ID_instantiate.
+      exists ([],map_start (Some 0)), (ws', <[0:=[]]> vis, ms), [].
+      constructor => //.
+      eapply HR_host_step => //; by rewrite gmap_of_list_lookup in Hmods.
+    + iIntros (e2 σ2 efs HStep) "!>!>!>".
+      iMod "Hmask".
+      iModIntro.
+      destruct σ2 as [[ws2 vis2] ms2].
+      destruct e2 as [he2 we2].
+      destruct HStep as [HStep [-> ->]].
+      inversion HStep; subst; last by apply empty_no_reduce in H0.
+      (* It appears that we need more resources in the precondition, so as to update the wasm store at this point. *)
+      admit.
+      
+  - iSpecialize ("Hwp" $! (hs, ws, [::], empty_instance) ns κ κs nt).
+    iSpecialize ("Hwp" with "[$]").
+    iMod "Hwp" as "(%Hred & Hwp)".
+    iModIntro.
+    iSplit.
+    
+    + destruct s => //.
+      iPureIntro.
+      unfold language.reducible.
+      
+      exists [], (([::], [AI_invoke 0]): host_expr), (ws', <[ 0 := [::] ]> vis , ms), [].
+      unfold prim_step => /=.
+      repeat split => //.
+      replace [AI_invoke 0] with (map_start (Some 0)); last trivial.
+      eapply HR_host_step => //.
+      by rewrite gmap_of_list_lookup in Hmods.
+        
+    + iIntros ([hes' wes'] [[ws2 vis2] ms2] efs HStep).
+      destruct HStep as [HStep [-> ->]].
+      inversion HStep; subst; clear HStep.
+      (* Latter case is impossible *)
+      (*
+      iSpecialize ("Hwp" $! wes' (hs', ws2, [::], empty_instance) [::] with "[%]"); first by unfold iris.prim_step.
+      iMod "Hwp".
+      do 2 iModIntro.
+      iMod "Hwp".
+      iModIntro.
+      iMod "Hwp".
+      iModIntro.
+      iDestruct "Hwp" as "((Hwf & Hwt & Hwm & Hwg & Hwframe & Hmsize) & Hwp)".
+      iDestruct "Hwp" as (f) "(Hf & Hwp & ?)".
+      iFrame.
+      iSplit => //.
+      iApply "IH"; first by apply hwev_reduce_closed in H0.
+      iApply "Hwp".
+      by iApply "Hf".
+*)
+Admitted.
+      
+
+
+
+                   
 
 End Iris_host.
